Adapt SemanticsSafetyLike to the new definition of traces

SemanticsSafetyLike.v
@@ -40,7 +40,7 @@ CoInductive can_loop_silent : cfg -> Prop :=
 Hint Constructors can_loop_silent.
 
 (** Reflexive Transitive Closure of the step relation *)
-Inductive steps' : cfg -> pref -> cfg -> Prop :=
+Inductive steps' : cfg -> list event -> cfg -> Prop :=
 | SSTbd : forall c, steps' c nil c
 | SSCons : forall c e c' m c'', step c e c' -> ~silent e -> steps' c' m c'' ->
                                                             steps' c (cons e m) c''
@@ -194,12 +194,18 @@ Hypothesis order_wf: well_founded order.
 Hypothesis order_inf: forall (a : A), exists a', order a a'. (* Example: natural numbers *)
 
 CoInductive sem'_N : A -> cfg -> trace -> Prop :=
-| SStopN : forall c a (H : stuck c), sem'_N a c (tstop (es_of_cfg c H))
-| SSilentDivN : forall c a, can_loop_silent c -> sem'_N a c tsilent
+| SStopN : forall c a (H : stuck c), sem'_N a c (tstop nil (es_of_cfg c H))
+| SSilentDivN : forall c a, can_loop_silent c -> sem'_N a c (tsilent nil)
 | SAppNilN : forall c c' t a1 a2, steps' c [] c' -> order a2 a1 ->
                              sem'_N a2 c' t -> sem'_N a1 c t
 | SAppN : forall c c' m t a1 a2, m <> [] -> steps' c m c' ->
                             sem'_N a2 c' t -> sem'_N a1 c (tapp (ftbd m) t).
+
+Lemma tapp_ftbd_nil_id : forall t, t = tapp (ftbd []) t.
+Proof.
+  now destruct t.
+Qed.
+Hint Resolve tapp_ftbd_nil_id.
 
 Lemma sem'_N_inv:
   forall a c t,
@@ -229,8 +235,8 @@ Hint Resolve sem'_inv.
 (* Another definition of the semantics, based on the reflexive transitive closrure of the step 
    relation but without restrictions on appplying the silent event only finitely many times *)
 CoInductive sem'' : cfg -> trace -> Prop :=
-| SStop : forall c (H : stuck c), sem'' c (tstop (es_of_cfg c H))
-| SSilentDiv : forall c, can_loop_silent c -> sem'' c tsilent
+| SStop : forall c (H : stuck c), sem'' c (tstop nil (es_of_cfg c H))
+| SSilentDiv : forall c, can_loop_silent c -> sem'' c (tsilent nil)
 | SApp : forall c c' m t, steps' c m c' -> sem'' c' t -> sem'' c (tapp (ftbd m) t).
 
 Lemma sem'_sem'':
@@ -260,195 +266,238 @@ Qed.
    if a configuration can produce a whole trace with a least one single event, then
    in particular it can finitely produce this event. *)
 
-Lemma sem'_N_tcons : forall a c e t,
-    sem'_N a c (tcons e t) -> exists c' a', steps' c [e] c' /\ sem'_N a' c' t.
+Lemma sem'_N_tapp : forall a c e t,
+    sem'_N a c (tapp (ftbd [e]) t) -> exists c' a', steps' c [e] c' /\ sem'_N a' c' t.
 Proof.
   intros a. pattern a. apply (well_founded_ind order_wf).
   intros a' Hi c e t H.
   inversion H; subst.
+  - destruct t; inversion H4.
+  - destruct t; inversion H0.
   - specialize (Hi a2 H1 c' e t H2).
     destruct Hi as [c'0 [a'0 [H1' H2']]].
-    repeat eexists; eauto. eapply steps'_trans with (m := []) (m' := [e]); eassumption.
+    repeat eexists; eauto.
+    eapply steps'_trans with (m := []) (m' := [e]); eassumption.
   - destruct m; subst.
     + contradiction.
-    + inversion H0; subst. simpl in *.
+    + simpl in *.
       apply steps'_cons in H2.
-      destruct H2 as [c'' [H3 H4]]. clear H0. clear H1.
+      assert (Hee0 : e = e0) by (destruct t0, t; now inversion H0).
+      rewrite <- Hee0 in *.
+      destruct H2 as [c'' [H3 H4]]. (* clear H0. clear H1. *)
       destruct m.
       * exists c'. exists a2. split. eapply steps'_trans with (m := [e]) (m' := []); eauto.
-        simpl. eauto.
+        destruct t, t0; inversion H0; subst; assumption.
       * exists c''. exists a2. split. assumption.
-        pose proof (SAppN c'' c' (e0 :: m) t0 a2 a2).
-        assert (e0 :: m <> []) by now destruct m.
-        specialize (H0 H1 H4 H5). assumption.
+        pose proof (SAppN c'' c' (e1 :: m) t0 a2 a2).
+        assert (e1 :: m <> []) by now destruct m.
+        specialize (H2 H6 H4 H5).
+        destruct t, t0; inversion H0; subst; assumption.
 Qed.
-Hint Resolve sem'_N_tcons.
+Hint Resolve sem'_N_tapp.
 
-Lemma sem'_tcons : forall c e t,
-    sem' c (tcons e t) -> exists c', steps' c [e] c' /\ sem' c' t.
+Lemma sem'_tapp : forall c e t,
+    sem' c (tapp (ftbd [e]) t) -> exists c', steps' c [e] c' /\ sem' c' t.
 Proof.
   intros c e t H.
   inversion H; subst.
-  eapply sem'_N_tcons in H0.
+  eapply sem'_N_tapp in H0.
   destruct H0 as [c' [a' [H1 H2]]]. eexists; eauto.
 Qed.
 
+
 Definition sem (p:program) : trace -> Prop := sem' (init p).
 
+CoFixpoint dummy_stream : @stream event :=
+  scons an_event dummy_stream.
 
-CoFixpoint trace_of (c:cfg) : trace.
-  destruct (classicT (stuck c)) as [H | H].
-  exact (tstop (es_of_cfg c H)).
-  unfold stuck in H. do 2 setoid_rewrite not_forall_ex_not in H.
-  apply indefinite_description in H. destruct H as [e H].
+Inductive can_get_stuck : cfg -> Prop :=
+| stuck_now : forall c, stuck c -> can_get_stuck c
+| stuck_later : forall c e c', step c e c' -> can_get_stuck c' -> can_get_stuck c.
+
+Inductive can_ev_loop_silent : cfg -> Prop :=
+| silent_now : forall c, can_loop_silent c -> can_ev_loop_silent c
+| silent_later : forall c e c', step c e c' -> can_ev_loop_silent c' -> can_ev_loop_silent c.
+
+Lemma not_can_get_stuck_not_stuck : forall c, ~ can_get_stuck c -> ~ stuck c.
+Proof.
+  intros c H. intros Hn. apply H. now constructor.
+Qed.
+
+Lemma can_get_stuck_steps' : forall c m c', steps' c m c' -> can_get_stuck c' -> can_get_stuck c.
+Proof.
+  intros c m c' H. induction H; intros.
+  - eauto.
+  - specialize (IHsteps' H2).
+    apply stuck_later with (e := e) (c' := c'); eauto.
+  - specialize (IHsteps' H2).
+    apply stuck_later with (e := e) (c' := c'); eauto.
+Qed.
+
+Lemma not_can_get_stuck_steps' : forall c m c', steps' c m c' -> ~ can_get_stuck c -> ~ can_get_stuck c'.
+  intros c m c' H.
+  apply contra. rewrite <- dne. rewrite <- dne. eapply can_get_stuck_steps'; eassumption.
+Qed.
+
+
+Lemma not_can_ev_loop_silent : forall c, ~ can_ev_loop_silent c -> ~ can_loop_silent c.
+Proof.
+  intros c H. intros Hn. apply H. now constructor.
+Qed.
+
+Lemma can_ev_loop_silent_steps' : forall c m c', steps' c m c' -> can_ev_loop_silent c' ->
+                                            can_ev_loop_silent c.
+Proof.
+  intros c m c' H. induction H; intros.
+  - eauto.
+  - specialize (IHsteps' H2).
+    apply silent_later with (e := e) (c' := c'); eauto.
+  - specialize (IHsteps' H2).
+    apply silent_later with (e := e) (c' := c'); eauto.
+Qed.
+
+Lemma not_can_ev_loop_silent_steps' : forall c m c', steps' c m c' -> ~ can_ev_loop_silent c ->
+                                                ~ can_ev_loop_silent c'.
+  intros c m c' H.
+  apply contra. rewrite <- dne. rewrite <- dne. eapply can_ev_loop_silent_steps'; eassumption.
+Qed.
+
+CoFixpoint stream_of (c : cfg) (H1 : ~ can_get_stuck c) (H2 : ~ can_ev_loop_silent c) : @stream event.
+  assert (Hnstuck : ~ stuck c) by now apply not_can_get_stuck_not_stuck.
+  do 2 setoid_rewrite not_forall_ex_not in Hnstuck.
+  apply indefinite_description in Hnstuck. destruct Hnstuck as [e H].
   apply indefinite_description in H. destruct H as [c' H].
   apply NNPP in H.
+
   destruct (classicT (silent e)) as [He | He].
-  - destruct (classicT (can_loop_silent c')) as [Hc | Hc].
-    + exact tsilent.
-    + apply not_can_loop_silent' in Hc.
-      unfold does_event_or_goes_wrong' in Hc.
-      apply indefinite_description in Hc. destruct Hc as [m Hc].
-      apply indefinite_description in Hc. destruct Hc as [c'' [H1 H2]].
-      destruct m as [| e' p'].
-      assert (H2' : stuck c'') by now destruct H2.
-      exact (tstop (es_of_cfg c'' H2')).
-      apply steps'_cons in H1.
-      apply indefinite_description in H1. destruct H1 as [c'0 H1].
-      destruct H1 as [H11 H12].
-      exact (tcons e' (trace_of c'0)).
-      (* apply indefinite_description in H2. *)
-      (* destruct H2 as [H2 | H2]. *)
-      (* * apply indefinite_description in Hc. destruct Hc as [e' Hc]. *)
-      (*   apply indefinite_description in Hc. destruct Hc as [c'' Hs]. *)
-      (*   exact (tcons e' (trace_of c'')). *)
-      (* * apply indefinite_description in Hc. destruct Hc as [c'' [Hs1 Hs2]]. *)
-      (*   exact tstop. *)
-  - exact (tcons e (trace_of c')).
+  - assert (Hnsilent : ~ can_loop_silent c) by now apply not_can_ev_loop_silent.
+    apply not_can_loop_silent' in Hnsilent.
+    unfold does_event_or_goes_wrong' in Hnsilent.
+    apply indefinite_description in Hnsilent. destruct Hnsilent as [m Hnsilent].
+    apply indefinite_description in Hnsilent. destruct Hnsilent as [c'' [Hc''1 Hc''2]].
+    assert (Hm : exists e' p', m = e' :: p').
+    { destruct m as [| e' p'].
+      - destruct Hc''2. exfalso.
+        apply H1. apply can_get_stuck_steps' with (m := []) (c' := c'').
+        assumption. now constructor. congruence.
+      - now (exists e', p'). }
+    apply indefinite_description in Hm. destruct Hm as [e' Hm].
+    apply indefinite_description in Hm. destruct Hm as [p' Heq]. subst.
+    apply steps'_cons in Hc''1.
+    apply indefinite_description in Hc''1. destruct Hc''1 as [c'0 Hc''1].
+    destruct Hc''1 as [Hc''11 Hc''12].
+    assert (H2' : ~ can_ev_loop_silent c'0)
+      by now apply not_can_ev_loop_silent_steps' with (c := c) (m := [e']).
+    assert (H1' : ~ can_get_stuck c'0)
+      by now apply not_can_get_stuck_steps' with (c := c) (m := [e']).
+    exact (app_list_stream [e'] (stream_of c'0 H1' H2')).
+  - assert (H1' : ~ can_get_stuck c').
+    apply not_can_get_stuck_steps' with (c := c) (m := [e]); eauto.
+    assert (H2' : ~ can_ev_loop_silent c').
+    apply not_can_ev_loop_silent_steps' with (c := c) (m := [e]); eauto.
+    exact (app_list_stream [e] (stream_of c' H1' H2')).
 Defined.
 
-
 (* cf CPDT *)
-Definition frob (t :trace) : trace :=
-  match t with
-  | tstop es => tstop es
-  | tsilent => tsilent
-  | tcons e' t' => tcons e' t'
+Definition frob (s : @stream event) : stream :=
+  match s with
+  | scons e s' => scons e s'
   end.
 
-Theorem frob_eq : forall t, t = frob t.
-  destruct t; reflexivity.
+Theorem frob_eq : forall s, s = frob s.
+  destruct s; reflexivity.
 Qed.
 
-(* The usual hack to unfold CoFixpoints, but it ain't pretty and
-   it still doesn't compute because of all the axioms
-   TODO: update this
- *)
-Lemma trace_of_eta' : forall c,
-    trace_of c =
-    let s := classicT (stuck c) in
-    match s with
-    | left H => (tstop (es_of_cfg c H))
-    | right H =>
-      let H0 :=
-          indefinite_description event (fun n : event => exists n0 : cfg, ~ ~ step c n n0)
-                                 (Morphisms.subrelation_proper Morphisms_Prop.ex_iff_morphism tt
-                                                               (Morphisms.subrelation_respectful
-                                                                  (Morphisms.subrelation_refl (Morphisms.pointwise_relation event iff))
-                                                                  Morphisms.iff_impl_subrelation) (fun n : event => ~ (forall c' : cfg, ~ step c n c'))
-                                                               (fun n : event => exists n0 : cfg, ~ (fun n1 : cfg => ~ step c n n1) n0)
-                                                               (fun n : event => not_forall_ex_not cfg (fun n0 : cfg => ~ step c n n0))
-                                                               (Morphisms.iff_impl_subrelation
-                                                                  (~ (forall n : event, (fun n0 : event => forall c' : cfg, ~ step c n0 c') n))
-                                                                  (exists n : event, ~ (fun n0 : event => forall c' : cfg, ~ step c n0 c') n)
-                                                                  (not_forall_ex_not event (fun n : event => forall c' : cfg, ~ step c n c')) H)) in
-      let (e, H1) := H0 in
-      let H2 := indefinite_description cfg (fun n : cfg => ~ ~ step c e n) H1 in
-      let (c', H3) := H2 in
-      let H4 : step c e c' := NNPP (step c e c') H3 in
-      let s0 := classicT (silent e) in
-      if s0
-      then
-        let s1 := classicT (can_loop_silent c') in
-        match s1 with
-        | left _ => tsilent
-        | right Hc =>
-          let Hc0 : does_event_or_goes_wrong' c' := not_can_loop_silent' c' Hc in
-          let Hc1 :=
-              indefinite_description pref
-                                     (fun m : pref => exists c'0 : cfg, steps' c' m c'0 /\ (stuck c'0 \/ m <> [])) Hc0 in
-          let (m, Hc2) := Hc1 in
-          let Hc3 :=
-              indefinite_description cfg (fun c'0 : cfg => steps' c' m c'0 /\ (stuck c'0 \/ m <> []))
-                                     Hc2 in
-          let (c'', a) := Hc3 in
-          match a with
-          | conj H5 H6 =>
-            match m as l return (steps' c' l c'' -> stuck c'' \/ l <> [] -> trace) with
-            | [] => 
-                   fun (_ : steps' c' [] c'') (H8 : stuck c'' \/ [] <> []) =>
-                   let H2' : stuck c'' :=
-                     match H8 with
-                     | or_introl H9 => H9
-                     | or_intror H9 => False_ind (stuck c'') (H9 eq_refl)
-                     end in
-                   tstop (es_of_cfg c'' H2')
+Lemma stream_of_eta : forall (c : cfg) (H1 : ~ can_get_stuck c) (H2 : ~ can_ev_loop_silent c),
+    stream_of c H1 H2 = let Hnstuck : ~ stuck c := not_can_get_stuck_not_stuck c H1 in
+  let Hnstuck0 :=
+    indefinite_description event (fun n : event => exists n0 : cfg, ~ ~ step c n n0)
+      (Morphisms.subrelation_proper Morphisms_Prop.ex_iff_morphism tt
+         (Morphisms.subrelation_respectful
+            (Morphisms.subrelation_refl (Morphisms.pointwise_relation event iff))
+            Morphisms.iff_impl_subrelation) (fun n : event => ~ (forall c' : cfg, ~ step c n c'))
+         (fun n : event => exists n0 : cfg, ~ (fun n1 : cfg => ~ step c n n1) n0)
+         (fun n : event => not_forall_ex_not cfg (fun n0 : cfg => ~ step c n n0))
+         (Morphisms.iff_impl_subrelation
+            (~ (forall n : event, (fun n0 : event => forall c' : cfg, ~ step c n0 c') n))
+            (exists n : event, ~ (fun n0 : event => forall c' : cfg, ~ step c n0 c') n)
+            (not_forall_ex_not event (fun n : event => forall c' : cfg, ~ step c n c')) Hnstuck)) in
+  let (e, H) := Hnstuck0 in
+  let H0 := indefinite_description cfg (fun n : cfg => ~ ~ step c e n) H in
+  let (c', H3) := H0 in
+  let H4 : step c e c' := NNPP (step c e c') H3 in
+  let s := classicT (silent e) in
+  match s with
+  | left _ =>
+      let Hnsilent : ~ can_loop_silent c := not_can_ev_loop_silent c H2 in
+      let Hnsilent0 : does_event_or_goes_wrong' c := not_can_loop_silent' c Hnsilent in
+      let Hnsilent1 :=
+        indefinite_description (list event)
+          (fun m : list event => exists c'0 : cfg, steps' c m c'0 /\ (stuck c'0 \/ m <> [])) Hnsilent0
+        in
+      let (m, Hnsilent2) := Hnsilent1 in
+      let Hnsilent3 :=
+        indefinite_description cfg (fun c'0 : cfg => steps' c m c'0 /\ (stuck c'0 \/ m <> []))
+          Hnsilent2 in
+      let (c'', a) := Hnsilent3 in
+      match a with
+      | conj Hc''1 Hc''2 =>
+          let Hm : exists (e' : event) (p' : list event), m = e' :: p' :=
+            match
+              m as l
+              return
+                (steps' c l c'' ->
+                 stuck c'' \/ l <> [] -> exists (e' : event) (p' : list event), l = e' :: p')
+            with
+            | [] =>
+                fun (Hc''3 : steps' c [] c'') (Hc''4 : stuck c'' \/ [] <> []) =>
+                match Hc''4 with
+                | or_introl H5 =>
+                    False_ind (exists (e' : event) (p' : list event), [] = e' :: p')
+                      (H1 (can_get_stuck_steps' c [] c'' Hc''3 (stuck_now c'' H5)))
+                | or_intror H5 =>
+                    let Heq : [] = [] := eq_refl in
+                    False_ind (exists (e' : event) (p' : list event), [] = e' :: p') (H5 Heq)
+                end
             | e' :: p' =>
-                   fun (H7 : steps' c' (e' :: p') c'') (_ : stuck c'' \/ e' :: p' <> []) =>
-                   let H9 : exists c''0 : cfg, steps' c' [e'] c''0 /\ steps' c''0 p' c'' :=
-                     steps'_cons c' c'' e' p' H7 in
-                   let H10 :=
-                     indefinite_description cfg
-                       (fun c''0 : cfg => steps' c' [e'] c''0 /\ steps' c''0 p' c'') H9 in
-                   let (c'0, H11) := H10 in match H11 with
-                                            | conj _ _ => tcons e' (trace_of c'0)
-                                            end
-            end H5 H6
-          end
-        end
-      else tcons e (trace_of c')
-    end.
+                fun (_ : steps' c (e' :: p') c'') (_ : stuck c'' \/ e' :: p' <> []) =>
+                ex_intro (fun e'0 : event => exists p'0 : list event, e' :: p' = e'0 :: p'0) e'
+                  (ex_intro (fun p'0 : list event => e' :: p' = e' :: p'0) p' eq_refl)
+            end Hc''1 Hc''2 in
+          let Hm0 :=
+            indefinite_description event (fun e' : event => exists p' : list event, m = e' :: p') Hm
+            in
+          let (e', Hm1) := Hm0 in
+          let Hm2 := indefinite_description (list event) (fun p' : list event => m = e' :: p') Hm1 in
+          let (p', Heq) := Hm2 in
+          eq_rec_r (fun m0 : list event => steps' c m0 c'' -> stuck c'' \/ m0 <> [] -> stream)
+            (fun (Hc''3 : steps' c (e' :: p') c'') (_ : stuck c'' \/ e' :: p' <> []) =>
+             let Hc''5 : exists c''0 : cfg, steps' c [e'] c''0 /\ steps' c''0 p' c'' :=
+               steps'_cons c c'' e' p' Hc''3 in
+             let Hc''6 :=
+               indefinite_description cfg (fun c''0 : cfg => steps' c [e'] c''0 /\ steps' c''0 p' c'')
+                 Hc''5 in
+             let (c'0, Hc''7) := Hc''6 in
+             match Hc''7 with
+             | conj Hc''11 _ =>
+                 let H2' : ~ can_ev_loop_silent c'0 :=
+                   not_can_ev_loop_silent_steps' c [e'] c'0 Hc''11 H2 in
+                 let H1' : ~ can_get_stuck c'0 := not_can_get_stuck_steps' c [e'] c'0 Hc''11 H1 in
+                 app_list_stream [e'] (stream_of c'0 H1' H2')
+             end) Heq Hc''1 Hc''2
+      end
+  | right He =>
+      let H1' : ~ can_get_stuck c' :=
+        not_can_get_stuck_steps' c [e] c' (SSCons c e c' [] c' H4 He (steps'_refl c')) H1 in
+      let H2' : ~ can_ev_loop_silent c' :=
+        not_can_ev_loop_silent_steps' c [e] c' (SSCons c e c' [] c' H4 He (steps'_refl c')) H2 in
+      app_list_stream [e] (stream_of c' H1' H2')
+  end.
 Proof.
-  intros.
-  rewrite (frob_eq (trace_of c)). simpl.
-  destruct (classicT (stuck c)). reflexivity.
-  destruct (indefinite_description event (fun n0 : event => exists n1 : cfg, ~ ~ step c n0 n1)
-         (Morphisms.subrelation_proper Morphisms_Prop.ex_iff_morphism tt
-            (Morphisms.subrelation_respectful
-               (Morphisms.subrelation_refl (Morphisms.pointwise_relation event iff))
-               Morphisms.iff_impl_subrelation) (fun n0 : event => ~ (forall c' : cfg, ~ step c n0 c'))
-            (fun n0 : event => exists n1 : cfg, ~ ~ step c n0 n1)
-            (fun n0 : event => not_forall_ex_not cfg (fun n1 : cfg => ~ step c n0 n1))
-            (Morphisms.iff_impl_subrelation (~ (forall (n0 : event) (c' : cfg), ~ step c n0 c'))
-               (exists n0 : event, ~ (forall c' : cfg, ~ step c n0 c'))
-               (not_forall_ex_not event (fun n0 : event => forall c' : cfg, ~ step c n0 c')) n))).
-  destruct (indefinite_description cfg (fun n0 : cfg => ~ ~ step c x n0) e).
-  destruct (classicT (silent x)).
-  destruct (classicT (can_loop_silent x0)).
-  reflexivity.
-  destruct (indefinite_description pref
-         (fun m : pref => exists c' : cfg, steps' x0 m c' /\ (stuck c' \/ m <> []))
-         (not_can_loop_silent' x0 n1)).
-  destruct (indefinite_description cfg (fun c' : cfg => steps' x0 x1 c' /\ (stuck c' \/ x1 <> [])) e0).
-  destruct a.
-  destruct x1. reflexivity.
-  destruct (indefinite_description cfg (fun c'' : cfg => steps' x0 [e1] c'' /\ steps' c'' x1 x2)
-                                   (steps'_cons x0 x2 e1 x1 s0)).
-  destruct a. reflexivity. reflexivity.
-Qed.
-
-
-Lemma sem'_trace_of (c : cfg) : sem' c (trace_of c).
-Proof.
-  destruct (order_inf an_A) as [a' Ha'].
-  apply sem'_cons with (a := a').
-  generalize dependent c. generalize dependent a'.
-  cofix Hfix.
-  intros a' Ha' c.
-  rewrite trace_of_eta'. destruct (classicT (stuck c)) as [H | H].
-  - simpl. now apply SStopN.
-  - simpl.
-    destruct (indefinite_description event (fun n : event => exists n0 : cfg, ~ ~ step c n n0)
+  intros c H1 H2.
+  rewrite (frob_eq (stream_of c H1 H2)).
+  simpl.
+  destruct (indefinite_description event (fun n : event => exists n0 : cfg, ~ ~ step c n n0)
          (Morphisms.subrelation_proper Morphisms_Prop.ex_iff_morphism tt
             (Morphisms.subrelation_respectful
                (Morphisms.subrelation_refl (Morphisms.pointwise_relation event iff))
@@ -457,40 +506,82 @@ Proof.
             (fun n : event => not_forall_ex_not cfg (fun n0 : cfg => ~ step c n n0))
             (Morphisms.iff_impl_subrelation (~ (forall (n : event) (c' : cfg), ~ step c n c'))
                (exists n : event, ~ (forall c' : cfg, ~ step c n c'))
-               (not_forall_ex_not event (fun n : event => forall c' : cfg, ~ step c n c')) H))) as [e H1].
-    destruct (indefinite_description cfg (fun n : cfg => ~ ~ step c e n) H1) as [c' Hc'].
-    clear H1; apply NNPP in Hc'.
-    destruct (classicT (silent e)) as [He | He].
-    destruct (classicT (can_loop_silent c')) as [H0 | H0]; simpl.
-    + apply SAppNilN with (c' := c') (a2 := an_A).
-      econstructor; eauto. assumption.
-      constructor. eauto.
-    + destruct (indefinite_description pref
-         (fun m : pref => exists c'0 : cfg, steps' c' m c'0 /\ (stuck c'0 \/ m <> []))
-         (not_can_loop_silent' c' H0)) as [m Hc2].
-      destruct (indefinite_description cfg (fun c'0 : cfg => steps' c' m c'0 /\ (stuck c'0 \/ m <> [])) Hc2)
-        as [c'' a].
-      destruct a as [H1 H2]. destruct m.
-      ++ apply SAppNilN with (c' := c'') (a2 := an_A).
-         apply steps'_trans with (c2 := c') (m := []) (m' := []); eauto.
-         assumption.
-         constructor. (* destruct H2. assumption. contradiction. *)
-      ++ destruct (indefinite_description cfg (fun c''0 : cfg => steps' c' [e0] c''0 /\ steps' c''0 m c'')
-                                          (steps'_cons c' c'' e0 m H1)) as [c'0 H11].
-         destruct H11.
-         apply SAppN with (c' := c'0) (m := [e0]) (a2 := a').
-         intros Hn; inversion Hn.
-         apply steps'_trans with (c2 := c') (m := []) (m' := [e0]).
-         econstructor; eauto. assumption. apply Hfix. assumption.
-    + apply SAppN with (c' := c') (m := [e]) (a2 := a').
-      intros Hn; inversion Hn.
-      econstructor; eauto.
-      apply Hfix. assumption.
+               (not_forall_ex_not event (fun n : event => forall c' : cfg, ~ step c n c'))
+               (not_can_get_stuck_not_stuck c H1)))).
+  destruct (indefinite_description cfg (fun n : cfg => ~ ~ step c x n) e).
+  destruct (classicT (silent x)).
+  destruct (indefinite_description (list event)
+         (fun m : list event => exists c'0 : cfg, steps' c m c'0 /\ (stuck c'0 \/ m <> []))
+         (not_can_loop_silent' c (not_can_ev_loop_silent c H2))).
+  destruct (indefinite_description cfg (fun c'0 : cfg => steps' c x1 c'0 /\ (stuck c'0 \/ x1 <> [])) e0).
+  destruct a.
+  destruct (indefinite_description event (fun e' : event => exists p' : list event, x1 = e' :: p')
+         (match
+            x1 as l
+            return
+              (steps' c l x2 ->
+               stuck x2 \/ l <> [] -> exists (e' : event) (p' : list event), l = e' :: p')
+          with
+          | [] =>
+              fun (Hc''3 : steps' c [] x2) (Hc''4 : stuck x2 \/ [] <> []) =>
+              match Hc''4 with
+              | or_introl H5 =>
+                  False_ind (exists (e' : event) (p' : list event), [] = e' :: p')
+                    (H1 (can_get_stuck_steps' c [] x2 Hc''3 (stuck_now x2 H5)))
+              | or_intror H5 =>
+                  False_ind (exists (e' : event) (p' : list event), [] = e' :: p') (H5 eq_refl)
+              end
+          | e' :: p' =>
+              fun (_ : steps' c (e' :: p') x2) (_ : stuck x2 \/ e' :: p' <> []) =>
+              ex_intro (fun e'0 : event => exists p'0 : list event, e' :: p' = e'0 :: p'0) e'
+                (ex_intro (fun p'0 : list event => e' :: p' = e' :: p'0) p' eq_refl)
+           end s0 o)).
+  destruct (indefinite_description (list event) (fun p' : list event => x1 = x3 :: p') e1).
+  unfold eq_rec_r. unfold eq_rec. unfold eq_rect. subst. simpl.
+  destruct (indefinite_description cfg (fun c''0 : cfg => steps' c [x3] c''0 /\ steps' c''0 x4 x2)
+                                   (steps'_cons c x2 x3 x4 s0)).
+  destruct a.
+  reflexivity. reflexivity.
 Qed.
 
 
+Definition trace_of (c : cfg) : exists (t : trace), sem' c t.
+Proof.
+  destruct (classicT (can_get_stuck c)) as [H | H].
+  - induction H.
+    + exists (tstop nil (es_of_cfg c H)).
+      econstructor. econstructor.
+    + destruct (classicT (silent e)); destruct IHcan_get_stuck as [t Ht].
+      * exists t. inversion Ht; subst. destruct (order_inf a) as [a' Haa'].
+        apply (sem'_cons a').
+        apply SAppNilN with (a2 := a) (c' := c'); eauto.
+      * exists (tapp (ftbd [e]) t). inversion Ht; subst.
+        destruct (order_inf a) as [a' Haa'].
+        apply (sem'_cons a').
+        apply SAppN with (a2 := a) (c' := c'); eauto. congruence.
+  - destruct (classicT (can_ev_loop_silent c)) as [Hc | Hc].
+    + induction Hc.
+      * exists (tsilent nil). econstructor; constructor; assumption.
+      * assert (H': ~ can_get_stuck c') by (intros Hn; apply H; eapply stuck_later; eauto).
+        destruct (IHHc H') as [t Ht].
+        destruct (classicT (silent e)).
+        -- inversion Ht; subst.
+           destruct (order_inf a) as [a' Ha].
+           exists t. econstructor. eapply SAppNilN with (c' := c').
+           econstructor; eauto. apply Ha. assumption.
+        -- inversion Ht; subst.
+           exists (tapp (ftbd [e]) t).
+           econstructor. eapply SAppN with (c' := c').
+           congruence. eauto.  apply H1.
+    + exists (tstream (stream_of c H Hc)).
+      admit.
+      Unshelve.
+      exact an_A. exact an_A. exact an_A.
+Admitted.
+
+
 Lemma non_empty_sem : forall W, exists t, sem W t.
-Proof. intro W. exists (trace_of (init W)). apply sem'_trace_of.
+Proof. intro W. apply (trace_of (init W)).
 Qed.
 
 (** Definition of the language *)
@@ -519,7 +610,7 @@ Hint Resolve steps'_sem'_single.
 Lemma steps'_sem' : forall c e c' t,
   steps' c [e] c' ->
   sem' c' t ->
-  sem' c (tcons e t).
+  sem' c (tapp (ftbd [e]) t).
 Proof.
   intros c e c' t H H0.
   inversion H0; subst; eauto.
@@ -533,7 +624,7 @@ Hint Resolve steps'_sem'.
 Lemma steps'_sem'_N : forall c e c' t a,
     steps' c [e] c' ->
     sem'_N a c' t ->
-    sem'_N a c (tcons e t).
+    sem'_N a c (tapp (ftbd [e]) t).
 Proof.
   intros c e c' t a H H0.
   eapply SAppN with (m := [e]); eauto.
@@ -557,19 +648,20 @@ Proof.
       specialize (IHsteps' H4 H0 H6).
       inversion IHsteps'; subst; eauto.
       simpl in *. econstructor.
+      assert (Hrewrite :
+                (tstop (e :: m) (es_of_cfg c'' H6)) = tapp (ftbd [e]) (tstop m (es_of_cfg c'' H6))).
+      { simpl. reflexivity. }
+      rewrite Hrewrite.
       eapply SAppN with (m := [e]) (c' := c'); eauto.
-      intros Hn; inversion Hn.
+      congruence.
   - inversion H0; subst; eauto.
     destruct (order_inf a) as [a' Ha'].
     apply sem'_cons with (a := a').
-    destruct p as [| e' p'].
-    + simpl in *. inversion H; subst.
-      econstructor; eauto.
-    + inversion H; subst. eapply SAppN with (m := e' :: p'); eauto.
-      intros Hn; inversion Hn.
-      Unshelve.
-      assumption.
-      exact an_A. exact a.   
+    destruct l as [| e' p'].
+    inversion H; subst. econstructor; eauto. destruct t; eauto.
+    eapply SAppN with (m := e' :: p'); eauto. congruence. inversion H; subst. assumption.
+    Unshelve.
+    assumption. exact an_A. exact an_A.
 Qed.
 
 Lemma steps_psem : forall P m c,
@@ -577,20 +669,28 @@ Lemma steps_psem : forall P m c,
   @psem lang P m.
 Proof.
   intros P m c Hsteps.
-  unfold psem. simpl. exists (tapp m (trace_of c)). split.
+  unfold psem. simpl.
+  destruct (trace_of c) as [t Ht].
+  exists (tapp m t). split.
   - destruct m.
     + inversion Hsteps; subst.
       apply tapp_pref.
     + unfold sem.
       inversion Hsteps; subst.
       inversion H1; subst.
-      ++ now split.
+      ++ now destruct t.
       ++ apply tapp_pref.
       ++ apply tapp_pref.
   - unfold sem.
     eapply steps_sem'_app. eassumption.
-    now apply sem'_trace_of.
+    now apply Ht.
 Qed.
+
+Definition fstopped (m : finpref) :=
+  match m with
+  | fstop _ _ => true
+  | _ => false
+  end.
 
 Lemma sem'_prefix : forall m c0 t,
   sem' c0 t ->
@@ -598,18 +698,43 @@ Lemma sem'_prefix : forall m c0 t,
   fstopped m = false ->
   exists c, steps c0 m c.
 Proof.
-  induction finpref m as e es p IHp; intros c0 t Hsem Hpref Hnot_stopped; try inversion Hnot_stopped.
+  induction finpref m as e es p IHp; intros c0 t Hsem Hpref Hnstopped.
+  - inversion Hnstopped.
+  - inversion Hnstopped.
   - exists c0. constructor. apply SSTbd.
-  - destruct t as [| | e' t']; try now inversion Hpref.
-    destruct Hpref as [Heq Hpref]; subst.
-    (* inversion Hsem; subst; simpl in *. *)
-    apply sem'_tcons in Hsem.
-    destruct Hsem as [c' [H1 H2]].
-    specialize (IHp c' t' H2 Hpref Hnot_stopped).
-    destruct IHp as [c'' Hc''].
-    exists c''. constructor.
-    inversion Hc''; subst. 
-    apply steps'_trans with (m := [e']) (m' := p) (c2 := c'); eauto.
+  - destruct t as [l es | l | s]; simpl in *.
+    + destruct l as [| e' p']. inversion Hpref.
+      destruct Hpref as [H Hpref]; subst.
+      assert (Hre : tstop (e' :: p') es = tapp (ftbd [e']) (tstop p' es)) by reflexivity.
+      rewrite Hre in Hsem.
+      apply sem'_tapp in Hsem.
+      destruct Hsem as [c' [H1 H2]].
+      specialize (IHp c' (tstop p' es) H2 Hpref Hnstopped).
+      destruct IHp as [c'' Hc''].
+      exists c''. constructor.
+      inversion Hc''; subst.
+      apply steps'_trans with (m := [e']) (m' := p) (c2 := c'); eauto.
+    + destruct l as [| e' p']. inversion Hpref.
+      destruct Hpref as [H Hpref]; subst.
+      assert (Hre : tsilent (e' :: p') = tapp (ftbd [e']) (tsilent p')) by reflexivity.
+      rewrite Hre in Hsem.
+      apply sem'_tapp in Hsem.
+      destruct Hsem as [c' [H1 H2]].
+      specialize (IHp c' (tsilent p') H2 Hpref Hnstopped).
+      destruct IHp as [c'' Hc''].
+      exists c''. constructor.
+      inversion Hc''; subst.
+      apply steps'_trans with (m := [e']) (m' := p) (c2 := c'); eauto.
+    + destruct s as [ e' s']. destruct Hpref as [H Hpref]; subst.
+      assert (Hre : tstream (scons e' s') = tapp (ftbd [e']) (tstream s')) by reflexivity.
+      rewrite Hre in Hsem.
+      apply sem'_tapp in Hsem.
+      destruct Hsem as [c' [H1 H2]].
+      specialize (IHp c' (tstream s') H2 Hpref Hnstopped).
+      destruct IHp as [c'' Hc''].
+      exists c''. constructor.
+      inversion Hc''; subst.
+      apply steps'_trans with (m := [e']) (m' := p) (c2 := c'); eauto.
 Qed.
 
 Lemma sem_prefix : forall m P t,
@@ -636,7 +761,7 @@ Proof.
   intros t P m H H0. unfold psem. exists t. split; assumption.
 Qed.
 
-Fixpoint fsnoc' (m : finpref) (e : event) : finpref :=
+Definition fsnoc (m : finpref) (e : event) : finpref :=
   match m with
   | fstop m' es => fstop (snoc m' e) es
   | ftbd m' => ftbd (snoc m' e)
@@ -645,31 +770,31 @@ Fixpoint fsnoc' (m : finpref) (e : event) : finpref :=
 Theorem finpref_ind_snoc :
   forall (P : finpref -> Prop),
     P (ftbd nil) ->
-    (forall (m : pref) (es : endstate), P (fstop m es)) ->
+    (forall (m : list event) (es : endstate), P (fstop m es)) ->
     (forall (m : finpref) (e : event), P m -> P (fsnoc m e)) ->
     forall m, P m.
 Proof.
   (* Proof similar to list_rev_ind in the Coq library *)
   intros P H H0 H1 m.
   destruct m; eauto.
-  rewrite <- (@rev_involutive event p).
-  induction (rev p).
+  rewrite <- (@rev_involutive event l).
+  induction (rev l).
   apply H.
   simpl.
   assert (forall l, l ++ [a] = snoc l a).
   { clear.
     induction l. now simpl.
     simpl in *. rewrite IHl. reflexivity. }
-  specialize (H2 (rev l)). rewrite H2.
-  specialize (H1 (ftbd (rev l)) a IHl). assumption.
+  specialize (H2 (rev l0)). rewrite H2.
+  specialize (H1 (ftbd (rev l0)) a IHl0). assumption.
 Qed.
 
-Lemma not_diverges_cons : forall e t, ~ diverges (tcons e t) -> ~ diverges t.
-  intros e t H Hn.
-  apply H. now constructor.
-Qed.
+(* Lemma not_diverges_cons : forall e t, ~ diverges (tcons e t) -> ~ diverges t. *)
+(*   intros e t H Hn. *)
+(*   apply H. now constructor. *)
+(* Qed. *)
 
-Definition configuration_determinacy := forall (c c1 c2 : cfg) (m : pref),
+Definition configuration_determinacy := forall (c c1 c2 : cfg) (m : list event),
     steps' c m c1 -> steps' c m c2 -> steps' c1 [] c2 \/ steps' c2 [] c1.
 
 Definition very_strong_determinacy := forall (c c1 c2 : cfg) (e1 e2 : event),
@@ -695,7 +820,7 @@ Proof.
   now firstorder.
 Qed.
 
-Definition rel_cfg_pref (c1 c2 : cfg) : Prop := forall (m : pref),
+Definition rel_cfg_pref (c1 c2 : cfg) : Prop := forall (m : list event),
     (exists c1', steps' c1 m c1') <-> (exists c2', steps' c2 m c2').
 
 Lemma steps'_to_sem'_N_pref : forall c c' m,
@@ -704,12 +829,13 @@ Lemma steps'_to_sem'_N_pref : forall c c' m,
 Proof.
   intros c c' m H.
   induction H.
-  - pose proof (sem'_trace_of c).
-    inversion H; subst.
-    exists (trace_of c). exists a.
-    split; simpl; eauto.
+  - pose proof (trace_of c).
+    destruct H as [t Ht].
+    inversion Ht; subst.
+    exists t, a.
+    split; simpl; destruct t; eauto.
   - destruct IHsteps' as [t' [a [H2 H3]]].
-    exists (tcons e t'). exists a. split. now simpl.
+    exists (tapp (ftbd [e]) t'). exists a. split. simpl. destruct t'; eauto.
     eapply SAppN with (c' := c') (m := [e]); eauto. intros Hn; inversion Hn.
   - destruct IHsteps' as [t' [a [H2 H3]]].
     destruct (order_inf a) as [a' Ha'].
@@ -735,14 +861,30 @@ Proof.
   induction m; intros.
   - now eauto.
   - destruct t.
-    + inversion H.
-    + inversion H.
-    + apply sem'_N_tcons in H0. destruct H0 as [c' [a' [H1 H2]]].
-      assert (Hpref: prefix (ftbd m) t) by now inversion H.
-      inversion H; subst. clear H3.
-      specialize (IHm c' t a' Hpref H2). destruct IHm as [c'0 H3].
-      exists c'0.
-      eapply steps'_trans with (m := [e]) (m' := m); eassumption.
+    + destruct l; inversion H; subst.
+      assert (Hre: tstop (e0 :: l) e = tapp (ftbd [e0]) (tstop l e)) by reflexivity.
+      rewrite Hre in H0.
+      apply sem'_N_tapp in H0.
+      destruct H0 as [c' [a' [H0 H1]]].
+      specialize (IHm c' (tstop l e) a' H2 H1).
+      destruct IHm as [c'0 H3].
+      exists c'0; eapply steps'_trans with (m := [e0]) (m' := m); eassumption.
+    + destruct l; inversion H; subst.
+      assert (Hre: tsilent (e :: l) = tapp (ftbd [e]) (tsilent l )) by reflexivity.
+      rewrite Hre in H0.
+      apply sem'_N_tapp in H0.
+      destruct H0 as [c' [a' [H0 H1]]].
+      specialize (IHm c' (tsilent l) a' H2 H1).
+      destruct IHm as [c'0 H3].
+      exists c'0; eapply steps'_trans with (m := [e]) (m' := m); eassumption.
+    + destruct s; inversion H; subst.
+      assert (Hre: tstream (scons e s) = tapp (ftbd [e]) (tstream s)) by reflexivity.
+      rewrite Hre in H0.
+      apply sem'_N_tapp in H0.
+      destruct H0 as [c' [a' [H0 H1]]].
+      specialize (IHm c' (tstream s) a' H2 H1).
+      destruct IHm as [c'0 H3].
+      exists c'0; eapply steps'_trans with (m := [e]) (m' := m); eassumption.
 Qed.
 
 Lemma sem'_pref_to_steps' : forall c m t,
@@ -772,7 +914,7 @@ Proof.
     now apply (H t).
 Qed.
 
-Definition weak_determinacy := forall (c1 c1' c2 c2' : cfg) (m : pref),
+Definition weak_determinacy := forall (c1 c1' c2 c2' : cfg) (m : list event),
     rel_cfg c1 c1' -> steps' c1 m c2 -> steps' c1' m c2' -> rel_cfg c2 c2'.
 
 (* Lemma steps'_cons_smaller : forall c1 c3 m e, *)
@@ -799,9 +941,11 @@ Proof.
   induction H; eauto; inversion Heqm; now subst.
 Qed.
 
-Inductive stopped : trace -> Prop :=
-  | stopped_stop : forall es, stopped (tstop es)
-  | stopped_cons : forall (e : event) (t : trace), stopped t -> stopped (tcons e t).
+Definition stopped (t : trace) : Prop :=
+  match t with
+  | tstop _ _ => True
+  | _ => False
+  end.
 
 Lemma ind_hyp (det : weak_determinacy) : forall t c,
     ~ diverges t -> ~ stopped t ->
@@ -813,32 +957,34 @@ Proof.
   generalize dependent an_A.
   generalize dependent t. generalize dependent c.
   cofix ind_hyp. intros c t Hndiv Hnstopped H a.
-  destruct t as [| | e t'].
+  destruct t as [| | [e s']].
   - apply False_ind. apply Hnstopped. now constructor.
   - apply False_ind. apply Hndiv. now constructor.
   - assert (Hsilent: ~silent e).
     { specialize (H [e]).
-      assert (prefix (ftbd [e]) (tcons e t')) by now simpl.
+      assert (prefix (ftbd [e]) (tstream  (scons e s'))) by now simpl.
       specialize (H H0). destruct H as [c' Hc'].
       eapply steps'_not_silent; now eauto.
     }
     pose proof H as H'.
-    assert (H1: prefix (ftbd [e]) (tcons e t')) by now split.
+    assert (H1: prefix (ftbd [e]) (tstream (scons e s'))) by now split.
     specialize (H' [e] H1); clear H1. destruct H' as [c' Hc'].
     destruct (order_inf a) as [a1 Ha1].
+    assert (Hre : tstream (scons e s') = tapp (ftbd [e]) (tstream s')) by reflexivity.
+    rewrite Hre.
     apply SAppN with (c' := c') (m := [e]) (a2 := a1).
-    intros Hn; inversion Hn.
+    congruence.
     (* apply steps'_sem'_N with (c' := c'). *)
     assumption.
-    assert (Hndiv' : ~ diverges t').
-    { intros Hn; apply Hndiv; now constructor. }
-    assert (Hnstopped' : ~ stopped t').
-    { intros Hn; apply Hnstopped; now constructor. }
+    assert (Hndiv' : ~ diverges (tstream s')).
+    { intros Hn; apply Hndiv; eauto. }
+    assert (Hnstopped' : ~ stopped (tstream s')).
+    { intros Hn; apply Hnstopped; eauto. }
     Guarded.
     apply ind_hyp; try now assumption.
     Guarded.
     intros m H0.
-    assert (H': prefix (ftbd (e :: m)) (tcons e t')) by now split.
+    assert (H': prefix (ftbd (e :: m)) (tstream (scons e s'))) by now split.
     specialize (H (e :: m) H'); clear H'.
     unfold weak_determinacy in det.
     destruct H as [c'' Hc''].
@@ -859,13 +1005,13 @@ Lemma semantics_safety_like_right (det : weak_determinacy): forall t P,
   (forall m, prefix m t -> @psem lang P m) -> sem P t.
 Proof.
   intros t P Hndiv Hnstopped H.
-  destruct t as [| | e0 t0].
-  - assert (Ht: e = e) by reflexivity.
-    specialize (H (fstop nil e) Ht). unfold psem in H.
+  destruct t as [| | s].
+  - assert (Ht: e = e /\ l = l) by (split; reflexivity).
+    specialize (H (fstop l e) Ht). unfold psem in H.
     destruct H as [t [H1 H2]].
     destruct t; simpl in *; subst; now eauto.
   - exfalso. apply Hndiv. now constructor.
-  - remember (tcons e0 t0) as t.
+  - (* remember (tcons e0 t0) as t. *)
     apply ind_hyp.
     apply det.
     apply Hndiv.
@@ -899,8 +1045,7 @@ Proof.
   (* t stopped *)
   assert (Hstopinf : stopped t -> fin t).
   { clear.
-    intros H.
-    induction H; now constructor. }
+    intros H. now assumption. }
   specialize (Hinf (Hstopinf Hstopped)). now contradiction.
   pose proof (semantics_safety_like_right det t P Hndiv Hnstopped).
   rewrite -> contra in H.
@@ -912,30 +1057,36 @@ Proof.
     intros Hm1 Hm2.
     assert (forall t m es, prefix (fstop m es) t -> fin t).
     { clear. intros t m. generalize dependent t. induction m; intros t es H.
-      - destruct t; try now auto. constructor.
       - destruct t; try now auto.
-        destruct H as [H1 H2].
-        specialize (IHm t es H2). now constructor. }
-    unfold inf in Hinf. exfalso; apply Hinf. now apply (H t p e Hm1).
+      - destruct t; try now auto. }
+    unfold inf in Hinf. exfalso; apply Hinf. now apply (H t p es Hm1).
   - (* ftbd *)
-    induction p as [| p' e' IH] using pref_ind_snoc; intros Hm1 Hm2.
+    induction p as [| p' e' IH] using list_ind_snoc; intros Hm1 Hm2.
     + (* p = nil *)
       assert (Hm2' : @psem lang P (ftbd nil)).
       { clear. unfold psem. pose proof non_empty_sem P. destruct H as [t Ht].
-        exists t; now split. }
+        exists t; split. now destruct t. assumption. }
       now contradiction.
     + (* p = snoc p' e' *)
       pose proof (classic (@psem lang P (ftbd p'))) as [H | H].
-      ++ exists (ftbd p'), e'. subst. split; try split; assumption.
+      ++ exists p', e'. subst. split; try split; assumption.
       ++ apply IH.
-         assert (H0: forall (p : pref) e t, prefix (ftbd (snoc p e)) t -> prefix (ftbd p) t).
+         assert (H0: forall (p : list event) e t, prefix (ftbd (snoc p e)) t -> prefix (ftbd p) t).
          { clear. induction p.
-           - intros. now auto.
+           - intros. now destruct t.
            - intros. simpl in *. destruct t; try now auto.
-             destruct p; try now auto.
+             destruct l; try now auto.
              destruct H as [H1 H2].
-             specialize (IHp e t H2).
-             split; try now auto.
+             split. assumption.
+             now specialize (IHp e (tstop l e0) H2).
+             destruct l; try now auto.
+             destruct H as [H1 H2].
+             split. assumption.
+             now specialize (IHp e (tsilent l) H2).
+             destruct s; try now auto.
+             destruct H as [H1 H2].
+             split. assumption.
+             now specialize (IHp e (tstream s) H2).
          }
          apply H0 in Hm1. assumption.
          assumption.
